src/polyfix.lean
@@ -1,0 +1,31 @@
+import polycodable
+
+variables {α β : Type*}
+def fix_bounded_iter (f : α → β ⊕ α) : ℕ → α → option β
+| 0 x := none
+| (n + 1) x := match f x with
+  | (sum.inl y) := some y
+  | (sum.inr x') := fix_bounded_iter n x'
+end
+
+lemma fix_eq_fix_bounded {f : α → β ⊕ α} {x : α} {y : β} {i : ℕ}
+  (h : y ∈ fix_bounded_iter f i x) : y ∈ pfun.fix (f : α →. β ⊕ α) x :=
+begin
+  induction i with i ih generalizing x,
+  { simp [fix_bounded_iter] at h, contradiction, },
+  cases H : f x with vl vr,
+  { apply pfun.fix_stop, simp [fix_bounded_iter, H] at h ⊢, exact h.symm, },
+  specialize ih (by simpa [fix_bounded_iter, H, ← option.mem_def] using h),
+  rw [@comm _ (=), ← part.mem_some_iff, ← pfun.coe_val] at H,
+  rwa pfun.fix_fwd _ _ H,
+end
+
+section poly
+variables [polycodable α] [polycodable β]
+
+abbreviation encode_sizeof (x : α) := (polycodable.encode x).sizeof
+
+-- lemma polytime_fix_bounded (p : polynomial ℕ) (f : α → β ⊕ α) (g : α → β)
+--   (hf : ∀ x, g x ∈ fix_bounded_iter f (p.eval (encode_sizeof x)) x) : polytime_fun f → polytime_fun g :=
+
+end poly
